Coinductive, better definition of bisim

src/Concurrent/BarbedBisim.v
@@ -110,11 +110,6 @@ end.
 (* Definition isUsed (ι : PID) (Π : ProcessPool) : Prop :=
   exists ι' p, Π ι' = Some p /\ In ι (usedPidsProc p). *)
 
-(* If we only consider things in the ether: *)
-Definition isUsed (ι : PID) (n : Ether) : Prop :=
-  exists ι', (* (n ι ι' <> [])%type \/  *)(n ι' ι <> [])%type.
-(*                  ^------- only the target is considered, not the source *)
-
 (* Definition isUnTaken (ι : PID) (Π : ProcessPool) : Prop :=
   Π ι = None /\ isUsed ι Π. *)
 
@@ -128,57 +123,6 @@ Definition preCompatibleNodes (n1 n2 : Node) : Prop :=
 
 Definition symClos {T : Type} (R : T -> T -> Prop) : T -> T -> Prop :=
   fun t1 t2 => R t1 t2 /\ R t2 t1.
-
-Lemma isUsed_etherAdd :
-  forall ether ι ι' ι'' s,
-    isUsed ι ether ->
-    isUsed ι (etherAdd ι' ι'' s ether).
-Proof.
-  intros. unfold etherAdd, update. unfold isUsed. destruct H as [ι'0 H].
-  * exists ι'0. repeat break_match_goal; eqb_to_eq; subst; auto.
-    intro H0; apply length_zero_iff_nil in H0; rewrite app_length in H0.
-    simpl in H0; lia.
-Qed.
-
-Lemma isUsed_etherAdd_rev :
-  forall ether ι ι' ι'' s,
-    isUsed ι (etherAdd ι' ι'' s ether) ->
-    ι'' <> ι ->
-    isUsed ι ether.
-Proof.
-  intros. unfold etherAdd, update in *. unfold isUsed.
-  destruct H as [ι'0 H].
-  repeat break_match_hyp; eqb_to_eq; subst; eexists; eauto.
-  Unshelve. exact ι.
-Qed.
-
-Lemma isUsed_etherPop :
-  forall {ether ι ι' ι'' s ether'},
-    isUsed ι ether ->
-    etherPop ι' ι'' ether = Some (s, ether') ->
-    isUsed ι ether' \/ ι = ι''.
-Proof.
-  intros. destruct H as [ι'0 H].
-  unfold etherPop in H0. break_match_hyp. congruence.
-  inv H0. unfold update.
-  destruct (Nat.eq_dec ι ι''); auto.
-  left. exists ι'0. repeat break_match_goal; eqb_to_eq; subst; try congruence.
-Qed.
-
-Lemma isUsed_etherPop_rev :
-  forall {ether ι ι' ι'' s ether'},
-    isUsed ι ether' ->
-    etherPop ι' ι'' ether = Some (s, ether') ->
-    isUsed ι ether.
-Proof.
-  intros. destruct H as [ι'0 H].
-  unfold etherPop in H0. break_match_hyp. congruence.
-  unfold isUsed.
-  inv H0. unfold update in *.
-  repeat break_match_hyp; eqb_to_eq; subst; try congruence.
-  all: eexists; eauto.
-  now rewrite Heql.
-Qed.
 
 Theorem compatibility_of_reduction :
   forall n n' a ι, n -[a | ι]ₙ-> n' ->
@@ -208,30 +152,6 @@ Proof.
       + simpl. assumption.
 Qed.
 
-Lemma processes_dont_die :
-  forall n n' l, n -[l]ₙ->* n' ->
-    forall ι, n.2 ι <> None -> n'.2 ι <> None.
-Proof.
-  intros. induction H; auto.
-  apply IHclosureNodeSem. clear IHclosureNodeSem H1. inv H.
-  all: simpl in *.
-  1-3: unfold update in *; break_match_hyp; auto; congruence.
-  * unfold update in *. clear H3.
-    repeat break_match_hyp; auto; eqb_to_eq; subst; try congruence.
-    - break_match_goal; congruence.
-    - break_match_goal; congruence.
-Qed.
-
-Corollary processes_dont_die_Some :
-  forall n n' l, n -[l]ₙ->* n' ->
-    forall ι p, n.2 ι = Some p -> exists p', n'.2 ι = Some p'.
-Proof.
-  intros.
-  epose proof (processes_dont_die _ _ _ H ι _).
-  Unshelve. 2: { intro D. rewrite D in H0. congruence. }
-  destruct (n'.2 ι). eexists. reflexivity.
-  congruence.
-Qed.
 
 Corollary compatibility_of_reductions :
    forall n n' l, n -[l]ₙ->* n' ->
@@ -248,16 +168,6 @@ Proof.
 Qed.
 
 
-(* NOTE!!!!!!!!
-   This depends on LEM!
-   TODO: reformalise ethers with maps!
-*)
-From Coq Require Import Logic.Classical.
-Proposition isUsed_dec :
-  forall ι ether, isUsed ι ether \/ ~isUsed ι ether.
-Proof.
-  intros. apply classic.
-Qed.
 
 Theorem compatibility_of_reduction_rev :
   forall n n' a ι, n -[a | ι]ₙ-> n' ->
@@ -296,25 +206,6 @@ Proof.
       + simpl. assumption.
 Qed.
 
-Lemma processes_dont_die_None :
-  forall l n n', n -[l]ₙ->* n' ->
-    forall ι, n'.2 ι = None -> n.2 ι = None.
-Proof.
-  induction l using list_length_ind.
-  destruct (length l) eqn:Hl; intros.
-  * apply length_zero_iff_nil in Hl; subst. inv H0. auto.
-  * pose proof Hl.
-    eapply eq_sym, last_element_exists in Hl as [l' [x Eq]]. subst.
-    apply closureNodeSem_trans_rev in H0 as [n0' [D1 D2]].
-    rewrite app_length in H2. simpl in *.
-    inv D2. inv H7.
-    eapply H in D1; eauto. lia. inv H5; simpl.
-    1-3: unfold update in *; simpl in *; break_match_goal; eqb_to_eq; try congruence; auto.
-    clear -H3 H1. simpl in *.
-    unfold update in *.
-    repeat break_match_hyp; eqb_to_eq; try congruence; auto.
-Qed.
-
 Corollary compatibility_of_reductions_rev :
    forall l n n', n -[l]ₙ->* n' ->
     forall ι,
@@ -347,38 +238,90 @@ Proof.
         apply in_or_app. simpl. right. rewrite H0. now constructor.
 Qed.
 
-Lemma no_spawn_included :
-  forall l n n', n -[l]ₙ->* n' ->
-    forall ι, ~In ι (PIDsOf spawnPIDOf l) ->
-      n.2 ι = None <-> n'.2 ι = None.
-Proof.
-  intros. induction H; auto.
-  split; auto.
-  unfold PIDsOf in H0; simpl in H0. fold (PIDsOf spawnPIDOf l) in H0.
-  apply not_in_app in H0 as [H0_1 H0_2]. apply IHclosureNodeSem in H0_2.
-  clear IHclosureNodeSem H1. inv H; simpl in *.
-  1-3: unfold update in *; break_match_goal; destruct H0_2; split; intro F; auto; try congruence.
-  1: now apply H1 in F.
-  1: now apply H2 in F.
-  1: destruct a; destruct H1 as [ | [ | ] ]; try congruence; simpl in *;
-     now apply H2 in F.
-  * clear H2 H3 H0. split; intro;
-    unfold update in *; repeat break_match_hyp; eqb_to_eq; subst; try congruence.
-    - exfalso. apply H0_1. now left.
-    - now apply H0_2 in H.
-    - break_match_goal; eqb_to_eq; congruence.
-    - now apply H0_2 in H.
-    - now apply H0_2 in H.
-Qed.
+Fixpoint overtakes {A : Type} (eq_dec :forall (a b : A), {a = b} + {a <> b}) (a b : A) (l : list A) : Prop :=
+  match l with
+  | [] => False
+  | x :: xs =>
+    match eq_dec a x with
+    | left _ => True
+    | right _ => match eq_dec b x with
+                 | left _ => False
+                 | right _ => overtakes eq_dec a b xs
+                 end
+    end
+  end.
 
+(* Lemma spawn_overtakes_send :
+  forall n n' l, n -[l]ₙ->* n' ->
+    forall ι, In ι (PIDsOf sendPIDOf l) -> In ι (PIDsOf spawnPIDOf l) ->
+      overtakes (ι, spawn) (ι, send) l. *)
 
 (* What if a new PID is targeted by a message ->
-   PID compatibility should also include sent messages *)
+   PID compatibility should also include sent messages 
 
+   The following definition is sufficient, because if both spawn and send
+   is present in the trace for some PID ι, then the spawn will happen first
+   always. If there is no spawn (only send) for ι, then this should hold for
+   the other trace.
+*)
 Definition reductionPreCompatibility (n1 n2 : Node) l l' :=
   Forall (fun x => ~isUnTaken x n2) (PIDsOf spawnPIDOf l) /\
-  (forall ι, n1.2 ι = None -> In ι (PIDsOf sendPIDOf l) ->
-        isUnTaken ι n2 /\ In ι (PIDsOf sendPIDOf l')).
+  (forall ι, n1.2 ι = None ->
+             In ι (PIDsOf sendPIDOf l) -> 
+             ~In ι (PIDsOf spawnPIDOf l) ->
+        n2.2 ι = None /\
+        In ι (PIDsOf sendPIDOf l') /\
+        ~In ι (PIDsOf spawnPIDOf l')).
+
+Lemma no_spawn_unTaken :
+  forall n n' l, n -[l]ₙ->* n' ->
+    forall ι, isUnTaken ι n ->
+      ~In ι (PIDsOf spawnPIDOf l).
+Proof.
+  intros n n' l H. induction H; intros; simpl.
+  * congruence.
+  * intro Hin. inv H; simpl in *.
+    - apply IHclosureNodeSem in Hin. assumption.
+      destruct H1. split; simpl in *.
+      + unfold update in *; break_match_goal; auto. congruence.
+      + now apply isUsed_etherAdd.
+    - apply IHclosureNodeSem in Hin. assumption.
+      destruct H1. split; simpl in *.
+      + unfold update in *; break_match_goal; auto. congruence.
+      + eapply isUsed_etherPop in H2 as [H2 | H2]; try eassumption.
+        subst. unfold update in H. now rewrite Nat.eqb_refl in H.
+    - assert (isUnTaken ι0 (ether, ι ↦ p' ∥ Π)). {
+        destruct H1; split; auto.
+        simpl in *. unfold update in *; break_match_goal; auto. congruence.
+      }
+      apply IHclosureNodeSem in H. apply H.
+      destruct a; auto. destruct H3 as [? | [? | ?]]; congruence.
+    - destruct Hin.
+      + clear H5. subst. destruct H1. simpl in *. congruence.
+      + clear H5. assert (isUnTaken ι0 (ether, ι' ↦ inl ([], r, emptyBox, [], false) ∥ ι ↦ p' ∥ Π)). {
+          destruct H1; split; auto.
+          simpl in *. unfold update in *.
+          repeat break_match_goal; auto; try congruence.
+          eqb_to_eq. subst. break_match_hyp; try congruence.
+        }
+        apply IHclosureNodeSem in H5. now apply H5.
+Qed.
+
+Lemma included_spawn :
+  forall (l : list (Action * PID)) (n n' : Node),
+  n -[ l ]ₙ->* n' ->
+    forall ι : PID, In ι (PIDsOf spawnPIDOf l) ->
+      n'.2 ι <> None.
+Proof.
+  intros l n n' H. induction H; intros.
+  * intro. inv H.
+  * inv H; simpl in *; try assumption.
+    1-3: apply IHclosureNodeSem; try assumption.
+    - firstorder; now subst.
+    - clear H5. destruct H1. 2: apply IHclosureNodeSem; try assumption.
+      subst. apply processes_dont_die with (ι := ι0) in H0; auto.
+      cbn. unfold update. now rewrite Nat.eqb_refl.
+Qed.
 
 Theorem reduction_preserves_preCompatibility :
   forall n1 n2, (* symClos *) preCompatibleNodes n1 n2 ->
@@ -399,13 +342,10 @@ Proof.
     - rewrite Forall_forall in H3. apply H3 in i. congruence.
     - eapply no_spawn_included in n. 2: eassumption. now rewrite n in H7'.
   * destruct_hyps.
-    apply H4 in H7. 2: assumption. destruct_hyps.
-    eapply compatibility_of_reductions in H1. 2: eassumption.
-    destruct H1.
-    - apply H1.
-    - unfold isUnTaken in H7. destruct_hyps.
-      apply H5 in H7. 2: assumption. destruct H7.
-      destruct H7. congruence.
+    destruct (in_dec Nat.eq_dec ι (PIDsOf spawnPIDOf l)).
+    - eapply included_spawn in H0. 2: eassumption. now destruct H6.
+    - apply (H4 _ H9 H7) in n. destruct_hyps.
+      apply (no_spawn_included _ _ _ H1) in H12. now apply H12.
 Qed.
 
 Corollary reduction_preserves_compatibility :
@@ -424,34 +364,87 @@ Proof.
     2-3: eassumption. all: eassumption.
 Qed.
 
-Definition barbedBisim (U : list PID) (S : Node -> Node -> Prop) :=
-  forall A B,
-    symClos preCompatibleNodes A B ->
-    S A B ->
-    (forall A' a ι,
+CoInductive barbedBisim (U : list PID) : Node -> Node -> Prop :=
+| is_bisim (A B : Node) :
+  symClos preCompatibleNodes A B ->
+  ether_wf A.1 -> ether_wf B.1 ->
+  (forall A' a ι,
       A -[a | ι]ₙ-> A' ->
         exists B' l,
           reductionPreCompatibility A B [(a,ι)] l /\
           reductionPreCompatibility B A l [(a,ι)] /\
-          B -[l]ₙ->* B' /\
-      S A' B') /\
-    (forall source dest,
+          B -[l]ₙ->* B' /\ barbedBisim U A' B') ->
+  (forall source dest,
       ~In dest U ->
       exists source' l B',
       B -[l]ₙ->* B' /\
-      list_biforall Srel (A.1 source dest) (B'.1 source' dest)) /\
-    (forall B' a ι,
+      list_biforall Srel (A.1 source dest) (B'.1 source' dest)) ->
+  (forall B' a ι,
       B -[a | ι]ₙ-> B' ->
         exists A' l,
           reductionPreCompatibility B A [(a,ι)] l /\
           reductionPreCompatibility A B l [(a,ι)] /\
           A -[l]ₙ->* A' /\
-      S A' B') /\
-    (forall source dest,
+      barbedBisim U A' B') ->
+  (forall source dest,
       ~In dest U ->
       exists source' l A',
       A -[l]ₙ->* A' /\
-      list_biforall Srel (B.1 source dest) (A'.1 source' dest)).
+      list_biforall Srel (B.1 source dest) (A'.1 source' dest)) ->
+  barbedBisim U A B
+.
+
+Theorem reductionPreCompatibility_refl A A' a ι:
+  A -[ a | ι ]ₙ-> A' ->
+  reductionPreCompatibility A A [(a, ι)] [(a, ι)].
+Proof.
+  split; intros.
+  * cbn. break_match_goal; auto. constructor; auto.
+    intro. destruct H0. destruct a; inv Heqo. inv H.
+    1: destruct H3 as [? | [? | ?]]; congruence.
+    simpl in *. congruence.
+  * cbn in H1. break_match_hyp; inv H1. 2: { inv H3. }
+    destruct a; inv Heqo. split; auto. split; auto.
+    now constructor.
+Qed.
+
+Corollary Srel_refl :
+  forall s, SIGCLOSED s -> Srel s s.
+Proof.
+  destruct s; simpl; auto.
+Qed.
+
+(* Co-induction test, this probably can be proven without it *)
+Theorem barbedBisim_refl :
+  forall U A, ether_wf A.1 -> barbedBisim U A A.
+Proof.
+  cofix H. intros.
+  constructor.
+  * unfold symClos, preCompatibleNodes.
+    split; intros ι H1; apply H1.
+  * assumption.
+  * assumption.
+  * intros. exists A', [(a, ι)]. split. 2: split.
+    - eapply reductionPreCompatibility_refl; eassumption.
+    - eapply reductionPreCompatibility_refl; eassumption.
+    - split. econstructor. eassumption. constructor.
+      apply H.
+      now pose proof (ether_wf_preserved A A' [(a, ι)] ltac:(econstructor;[eassumption|constructor]) H0).
+  * intros. exists source, [], A.
+    split. constructor. apply forall_biforall_refl.
+    specialize (H0 source dest). rewrite Forall_forall in *.
+    intros. apply Srel_refl. now apply H0.
+  * intros. exists B', [(a, ι)]. split. 2: split.
+    - eapply reductionPreCompatibility_refl; eassumption.
+    - eapply reductionPreCompatibility_refl; eassumption.
+    - split. econstructor. eassumption. constructor.
+      apply H.
+      now pose proof (ether_wf_preserved A B' [(a, ι)] ltac:(econstructor;[eassumption|constructor]) H0).
+  * intros. exists source, [], A.
+    split. constructor. apply forall_biforall_refl.
+    specialize (H0 source dest). rewrite Forall_forall in *.
+    intros. apply Srel_refl. now apply H0.
+Qed.
 
 Definition barbedExpansion (U : list PID) (S : Node -> Node -> Prop) :=
   forall (A B : Node), S A B ->
@@ -474,6 +467,14 @@ Definition barbedExpansion (U : list PID) (S : Node -> Node -> Prop) :=
     exists source' l A',
     A -[l]ₙ->* A' /\
     list_biforall Srel (B.1 source dest) (A'.1 source' dest)).
+
+Theorem barbedExpansion_transitive :
+  forall U S, barbedExpansion U S ->
+    forall A B C, S A B -> S B C -> S A C.
+Proof.
+  intros. apply H in H0. apply H in H1.
+  clear H. destruct_hyps.
+Qed.
 
 Definition barbedBisimUpTo (U : list PID) (S : Node -> Node -> Prop) :=
  barbedExpansion U S /\
