src/Concurrent/NodeSemantics.v
@@ -138,6 +138,63 @@ Proof.
   all: auto; try congruence.
 Qed.
 
+(* If we only consider things in the ether: *)
+Definition isUsed (ι : PID) (n : Ether) : Prop :=
+  exists ι', (* (n ι ι' <> [])%type \/  *)(n ι' ι <> [])%type.
+(*                  ^------- only the target is considered, not the source *)
+
+Lemma isUsed_etherAdd :
+  forall ether ι ι' ι'' s,
+    isUsed ι ether ->
+    isUsed ι (etherAdd ι' ι'' s ether).
+Proof.
+  intros. unfold etherAdd, update. unfold isUsed. destruct H as [ι'0 H].
+  * exists ι'0. repeat break_match_goal; eqb_to_eq; subst; auto.
+    intro H0; apply length_zero_iff_nil in H0; rewrite app_length in H0.
+    simpl in H0; lia.
+Qed.
+
+Lemma isUsed_etherAdd_rev :
+  forall ether ι ι' ι'' s,
+    isUsed ι (etherAdd ι' ι'' s ether) ->
+    ι'' <> ι ->
+    isUsed ι ether.
+Proof.
+  intros. unfold etherAdd, update in *. unfold isUsed.
+  destruct H as [ι'0 H].
+  repeat break_match_hyp; eqb_to_eq; subst; eexists; eauto.
+  Unshelve. exact ι.
+Qed.
+
+Lemma isUsed_etherPop :
+  forall {ether ι ι' ι'' s ether'},
+    isUsed ι ether ->
+    etherPop ι' ι'' ether = Some (s, ether') ->
+    isUsed ι ether' \/ ι = ι''.
+Proof.
+  intros. destruct H as [ι'0 H].
+  unfold etherPop in H0. break_match_hyp. congruence.
+  inv H0. unfold update.
+  destruct (Nat.eq_dec ι ι''); auto.
+  left. exists ι'0. repeat break_match_goal; eqb_to_eq; subst; try congruence.
+Qed.
+
+Lemma isUsed_etherPop_rev :
+  forall {ether ι ι' ι'' s ether'},
+    isUsed ι ether' ->
+    etherPop ι' ι'' ether = Some (s, ether') ->
+    isUsed ι ether.
+Proof.
+  intros. destruct H as [ι'0 H].
+  unfold etherPop in H0. break_match_hyp. congruence.
+  unfold isUsed.
+  inv H0. unfold update in *.
+  repeat break_match_hyp; eqb_to_eq; subst; try congruence.
+  all: eexists; eauto.
+  now rewrite Heql.
+Qed.
+
+
 Reserved Notation "n -[ a | ι ]ₙ-> n'" (at level 50).
 Inductive nodeSemantics : Node -> Action -> PID -> Node -> Prop :=
 (** sending any signal *)
@@ -166,7 +223,10 @@ Inductive nodeSemantics : Node -> Action -> PID -> Node -> Prop :=
 
 (** spawning processes *)
 | n_spawn Π (p p' : Process) v1 v2 l ι ι' ether r eff:
-  mk_list v2 = Some l -> (ι ↦ p ∥ Π) ι' = None ->
+  mk_list v2 = Some l ->
+  (ι ↦ p ∥ Π) ι' = None ->
+  ~isUsed ι' ether -> (* We can't model spawning such processes that receive
+                         already floating messages from the ether. *)
   create_result (IApp v1) l [] = Some (r, eff) ->
   p -⌈ASpawn ι' v1 v2⌉-> p'
 ->
