src/Concurrent/ProcessSemantics.v
@@ -220,10 +220,12 @@ Inductive processLocalSemantics : Process -> Action -> Process -> Prop :=
 (********** SIGNAL SENDING **********)
 (* message send *)
 | p_send ι v mb fs flag links source :
+  VALCLOSED v ->
   inl (FParams (ICall erlang send) [VPid ι] [] :: fs, RValSeq [v], mb, links, flag)
   -⌈ ASend source ι (SMessage v) ⌉-> inl (fs, RValSeq [v], mb, links, flag)
 (* exit, 2 parameters *)
 | p_exit fs v mb flag ι selfι links :
+  VALCLOSED v ->
   inl (FParams (ICall erlang exit) [VPid ι] [] :: fs, RValSeq [v], mb, links, flag) -⌈ ASend selfι ι (SExit v false) ⌉->
   inl (fs, RValSeq [ttrue], mb, links, flag)
 (* link *)
@@ -238,6 +240,7 @@ Inductive processLocalSemantics : Process -> Action -> Process -> Prop :=
   inl (fs, RValSeq [ok], mb, remove Nat.eq_dec ι links, flag)
 (* DEAD PROCESSES *)
 | p_dead ι selfι links reason:
+  VALCLOSED reason ->
   inr ((ι, reason) :: links) -⌈ASend selfι ι (SExit reason true)⌉-> inr links
 
 
